aneris/aneris_lang/state_interp/state_interp_free_ips_coh.v
@@ -17,23 +17,37 @@ Import RecordSetNotations.
 Section state_interpretation.
   Context `{!anerisG Mdl Σ}.
 
+  Definition ip_is_free (ip : ip_address) (σ : state) : Prop :=
+    state_heaps σ !! ip = None ∧ state_sockets σ !! ip = None.
+
   (** free_ips_coh *)
-  Lemma free_ips_coh_init ip ips σ :
-    ip ∉ ips →
-    state_heaps σ = {[ip:=∅]} →
-    state_sockets σ = {[ip:=∅]} →
-    state_ms σ = ∅ →
-    free_ips_auth ips ∗ free_ports_auth ∅ -∗ free_ips_coh σ.
+  Lemma free_ips_coh_init ips σ :
+    (∀ ip, ip ∈ ips → ip_is_free ip σ) →
+    free_ips_auth ips ∗ free_ports_auth ∅ -∗
+    free_ips_coh σ.
   Proof.
-    iIntros (? Hste Hsce ?) "[HipsCtx HPiu]".
+    iIntros (Hip) "[HipsCtx HPiu]".
     iExists _, _; iFrame.
-    rewrite Hste Hsce.
-    iPureIntro.
-    do 2 (split; try set_solver).
-    intros ip' ?. 
-    assert (ip ≠ ip') by set_solver.
-    rewrite !lookup_insert_ne //.
+    iPureIntro. set_solver.
   Qed.
+
+  (* (** free_ips_coh *) *)
+  (* Lemma free_ips_coh_init ip ips σ : *)
+  (*   ip ∉ ips → *)
+  (*   state_heaps σ = {[ip:=∅]} → *)
+  (*   state_sockets σ = {[ip:=∅]} → *)
+  (*   state_ms σ = ∅ → *)
+  (*   free_ips_auth ips ∗ free_ports_auth ∅ -∗ free_ips_coh σ. *)
+  (* Proof. *)
+  (*   iIntros (? Hste Hsce ?) "[HipsCtx HPiu]". *)
+  (*   iExists _, _; iFrame. *)
+  (*   rewrite Hste Hsce. *)
+  (*   iPureIntro. *)
+  (*   do 2 (split; try set_solver). *)
+  (*   intros ip' ?.  *)
+  (*   assert (ip ≠ ip') by set_solver. *)
+  (*   rewrite !lookup_insert_ne //. *)
+  (* Qed. *)
 
   Lemma free_ips_coh_free_ports_valid σ a Sn :
     state_sockets σ !! ip_of_address a = Some Sn → 
